proof/CCPD.alaChen/Generation.v
@@ -127,11 +127,11 @@ unfold lift in H ; simpl in H.
 injection H ; intros.
 exists t1 ; exists t2 ; split ; [auto | split ; auto].
 Qed.
-
+(*
 Lemma prod_no_kind : forall t G T, G |- t : T -> 
-  forall U V, t = Prod U V -> ~ (exists n, prod_target t n (Srt kind)).
+  forall U V, t = Prod U V -> ~ (exists n, prod_target t n (Srt kind)).*)
 
-Ltac doubleind t := induction t as [dH1] ; induction dH1 as [dH2].
+(*Ltac doubleind t := induction t as [dH1] ; induction dH1 as [dH2].*)
 
 Lemma prod_target_not_kind : forall t G T, G |- t : T -> 
   forall U V, t = Prod U V -> ~ (exists n, prod_target t n (Srt kind)).
