proof/CCPD.alaChen/Thinning.v
@@ -3,35 +3,35 @@ Require Import Reduction.
 Require Import LiftSubst.
 Require Import Env.
 Require Import CCPD.Types.
+Require Import Conv.
 
 Implicit Types i k m n p : nat.
 Implicit Type s : sort.
 Implicit Types A B M N T t u v : term.
 Implicit Types e f g : env.
 
-Lemma coerce_sort : forall e T U,   e |- T >> U ->
- forall s1 s2, e |- T : Srt s1 -> e |- U : Srt s2 -> s1 = s2.
+Lemma typ_weak_weak : forall A e t T, e |- t : T ->
+   forall n f, ins_in_env A n e f -> wf f -> 
+   f |- (lift_rec 1 t n) : (lift_rec 1 T n).
 Proof.
-  induction 1 ; intros.
-  
-
-
-  Lemma typ_weak_weak :
-   forall A e t T,
-   typ e t T ->
-   forall n f,
-   ins_in_env A n e f -> wf f -> typ f (lift_rec 1 t n) (lift_rec 1 T n).
-intros A e t T IHt.
-induction IHt using typ_mut with 
- (P := fun e t T => fun IHt : typ e t T =>
+intros A e t T IH.
+induction IH using typ_mut with 
+ (P := fun e t T => fun IH : typ e t T =>
    forall n f,
    ins_in_env A n e f -> wf f -> typ f (lift_rec 1 t n) (lift_rec 1 T n))
- (P0 := fun e T U => fun IHt : coerce e T U =>
-   forall s, e |- T : Srt s -> e |- U : Srt s ->
+ (P0 := fun e T U s => fun IH : coerce e T U s =>
    forall n f,
-   ins_in_env A n e f -> wf f -> coerce f (lift_rec 1 T n) (lift_rec 1 U n)) ;
-simpl in |- *; try simpl in IHIHt ; try simpl in IHIHt1 ; try simpl in IHIHt2 ; try simpl in IHIHt3 ; 
-try simpl in IHIHt4 ; intros; auto with coc core arith datatypes.
+   ins_in_env A n e f -> wf f -> f |- (lift_rec 1 T n) >> (lift_rec 1 U n) : s) ;
+   simpl in |- *; 
+   try simpl in IHIH ; 
+   try simpl in IHIH0 ; 
+   try simpl in IHIH1 ; 
+   try simpl in IHIH2 ; 
+   try simpl in IHIH3 ; 
+   try simpl in IHIH4 ; 
+   try simpl in IHIH5 ; 
+   try simpl in IHIH6 ; 
+   intros; auto with coc core arith datatypes.
 
 elim (le_gt_dec n0 n); intros; apply type_var;
  auto with coc core arith datatypes.
@@ -54,101 +54,11 @@ rewrite distr_lift_subst.
 apply type_app with (lift_rec 1 V n); auto with coc core arith datatypes.
 
 apply type_pair with s1 s2 ; auto with coc core arith datatypes.
-apply IHIHt3 ; auto with coc core arith datatypes.
+apply IHIH3 ; auto with coc core arith datatypes.
 apply wf_var with s1 ; auto with coc core arith datatypes.
 
 rewrite <- distr_lift_subst.
-apply IHIHt4 ; auto with coc core arith datatypes.
-
-cut (wf (lift_rec 1 T n :: f)).
-intro.
-apply type_prod with s1; auto with coc core arith datatypes.
-apply wf_var with s1; auto with coc core arith datatypes.
-
-cut (wf (lift_rec 1 T n :: f)).
-intro.
-apply type_sum with s1; auto with coc core arith datatypes.
-apply wf_var with s1; auto with coc core arith datatypes.
-
-cut (wf (lift_rec 1 T n :: f)).
-intro.
-apply type_subset ; auto with coc core arith datatypes.
-apply wf_var with set; auto with coc core arith datatypes.
-
-apply type_pi1 with (lift_rec 1 V (S n)) ; auto with coc.
-
-rewrite distr_lift_subst.
-simpl.
-apply type_pi2 with (lift_rec 1 U n); auto with coc.
-
-cut (wf (lift_rec 1 U n :: f)).
-intro.
-rewrite distr_lift_subst.
-apply type_let_in with (lift_rec 1 U n) s1 s2 ; auto with coc core.
-apply wf_var with s1 ; auto with coc core.
-
-apply type_conv with (lift_rec 1 U n) s; auto with coc core arith datatypes.
-apply IHIHt4 with s ; auto with coc.
-
-apply coerce_prod ; auto with coc.
-
-apply IHIHt with s ; auto with coc.
-
-apply wf_var with s.
-apply IHIHc1 ; auto with coc core.
-
-apply coerce_sum with s ; auto with coc.
-apply IHIHc4; auto with coc.
-apply wf_var with s.
-apply IHIHc2 ; auto with coc core.
-
-apply coerce_trans with (lift_rec 1 B n) s ; auto with coc core.
-
-
-Qed.
-
-  Lemma coerce_weak_weak :
-   forall A e T U,
-   e |- T >> U ->
-   forall n f,
-   ins_in_env A n e f -> wf f -> coerce f (lift_rec 1 T n) (lift_rec 1 U n).
-intros A e t T IHc.
-induction IHc using coerce_mut with 
- (P := fun e t T => fun IHt : typ e t T =>
-   forall n f,
-   ins_in_env A n e f -> wf f -> typ f (lift_rec 1 t n) (lift_rec 1 T n))
- (P0 := fun e T U => fun IHt : coerce e T U =>
-   forall n f,
-   ins_in_env A n e f -> wf f -> coerce f (lift_rec 1 T n) (lift_rec 1 U n)) ;
-simpl in |- *; try simpl in IHIHc ; try simpl in IHIHc0 ; try simpl in IHIHc1 ; try simpl in IHIHc2 ; try simpl in IHIHc3 ; 
-try simpl in IHIHc4 ; intros; auto with coc core arith datatypes.
-
-elim (le_gt_dec n0 n); intros; apply type_var;
- auto with coc core arith datatypes.
-elim i; intros.
-exists x.
-rewrite H1.
-unfold lift in |- *.
-rewrite simpl_lift_rec; simpl in |- *; auto with coc core arith datatypes.
-
-apply ins_item_ge with A n0 e; auto with coc core arith datatypes.
-
-apply ins_item_lt with A e; auto with coc core arith datatypes.
-
-cut (wf (lift_rec 1 T n :: f)).
-intro.
-apply type_abs with s1 s2 ; auto with coc core arith datatypes.
-apply wf_var with s1 ; auto with coc core arith datatypes.
-
-rewrite distr_lift_subst.
-apply type_app with (lift_rec 1 V n); auto with coc core arith datatypes.
-
-apply type_pair with s1 s2 ; auto with coc core arith datatypes.
-apply IHIHc1 ; auto with coc core arith datatypes.
-apply wf_var with s1 ; auto with coc core arith datatypes.
-
-rewrite <- distr_lift_subst.
-apply IHIHc2 ; auto with coc core arith datatypes.
+apply IHIH4 ; auto with coc core arith datatypes.
 
 cut (wf (lift_rec 1 T n :: f)).
 intro.
@@ -180,22 +90,170 @@ apply wf_var with s1 ; auto with coc core.
 apply type_conv with (lift_rec 1 U n) s; auto with coc core arith datatypes.
 
 apply coerce_prod with s ; auto with coc.
-apply IHIHc4; auto with coc.
+
+apply IHIH4 ; auto with coc core.
 apply wf_var with s.
-apply IHIHc1 ; auto with coc core.
+
+apply IHIH2 ; auto with coc core.
+apply IHIH5 ; auto with coc core.
+apply wf_var with s.
+apply IHIH3 ; auto with coc core.
+
+apply IHIH6 ; auto with coc core.
+apply wf_var with s.
+apply IHIH2 ; auto with coc core.
 
 apply coerce_sum with s ; auto with coc.
-apply IHIHc4; auto with coc.
-apply wf_var with s.
-apply IHIHc2 ; auto with coc core.
 
-apply coerce_trans with (lift_rec 1 B n) s ; auto with coc core.
+apply IHIH4 ; auto with coc.
+apply wf_var with s.
+apply IHIH3 ; auto with coc core.
+apply IHIH5 ; auto with coc core.
+apply wf_var with s.
+apply IHIH3 ; auto with coc core.
+
+apply IHIH6 ; auto with coc core.
+apply wf_var with s.
+apply IHIH2 ; auto with coc core.
+
+apply coerce_sub_l ; auto with coc core.
+apply IHIH0 ; auto with coc core.
+apply wf_var with set.
+eapply coerce_sort_l  ; auto with coc.
+
+apply coerce_sub_r ; auto with coc core.
+apply IHIH0 ; auto with coc core.
+apply wf_var with set.
+eapply coerce_sort_r  ; auto with coc.
+
+apply coerce_trans with (lift_rec 1 B n) ; auto with coc core.
 Qed.
 
+
+
+Lemma coerce_weak_weak : forall A e T U s, e |- T >> U : s ->
+  forall n f, ins_in_env A n e f -> wf f -> 
+  f |- (lift_rec 1 T n) >> (lift_rec 1 U n) : s.
+Proof.
+intros A e T U s IH.
+induction IH using coerce_mut with 
+ (P := fun e t T => fun IHt : typ e t T =>
+   forall n f,
+   ins_in_env A n e f -> wf f -> typ f (lift_rec 1 t n) (lift_rec 1 T n))
+ (P0 := fun e T U s => fun IHt : coerce e T U s =>
+   forall n f,
+   ins_in_env A n e f -> wf f -> coerce f (lift_rec 1 T n) (lift_rec 1 U n) s) ;
+   simpl in |- *; 
+   try simpl in IHIH ; 
+   try simpl in IHIH0 ; 
+   try simpl in IHIH1 ; 
+   try simpl in IHIH2 ; 
+   try simpl in IHIH3 ; 
+   try simpl in IHIH4 ; 
+   try simpl in IHIH5 ; 
+   try simpl in IHIH6 ; 
+   intros; auto with coc core arith datatypes.
+
+elim (le_gt_dec n0 n); intros; apply type_var;
+ auto with coc core arith datatypes.
+elim i; intros.
+exists x.
+rewrite H1.
+unfold lift in |- *.
+rewrite simpl_lift_rec; simpl in |- *; auto with coc core arith datatypes.
+
+apply ins_item_ge with A n0 e; auto with coc core arith datatypes.
+
+apply ins_item_lt with A e; auto with coc core arith datatypes.
+
+cut (wf (lift_rec 1 T n :: f)).
+intro.
+apply type_abs with s1 s2 ; auto with coc core arith datatypes.
+apply wf_var with s1 ; auto with coc core arith datatypes.
+
+rewrite distr_lift_subst.
+apply type_app with (lift_rec 1 V n); auto with coc core arith datatypes.
+
+apply type_pair with s1 s2 ; auto with coc core arith datatypes.
+apply IHIH1 ; auto with coc core arith datatypes.
+apply wf_var with s1 ; auto with coc core arith datatypes.
+
+rewrite <- distr_lift_subst.
+apply IHIH2 ; auto with coc core arith datatypes.
+
+cut (wf (lift_rec 1 T n :: f)).
+intro.
+apply type_prod with s1; auto with coc core arith datatypes.
+apply wf_var with s1; auto with coc core arith datatypes.
+
+cut (wf (lift_rec 1 T n :: f)).
+intro.
+apply type_sum with s1; auto with coc core arith datatypes.
+apply wf_var with s1; auto with coc core arith datatypes.
+
+cut (wf (lift_rec 1 T n :: f)).
+intro.
+apply type_subset ; auto with coc core arith datatypes.
+apply wf_var with set; auto with coc core arith datatypes.
+
+apply type_pi1 with (lift_rec 1 V (S n)) ; auto with coc.
+
+rewrite distr_lift_subst.
+simpl.
+apply type_pi2 with (lift_rec 1 U n); auto with coc.
+
+cut (wf (lift_rec 1 U n :: f)).
+intro.
+rewrite distr_lift_subst.
+apply type_let_in with (lift_rec 1 U n) s1 s2 ; auto with coc core.
+apply wf_var with s1 ; auto with coc core.
+
+apply type_conv with (lift_rec 1 U n) s; auto with coc core arith datatypes.
+
+apply coerce_prod with s ; auto with coc.
+
+apply IHIH4 ; auto with coc core.
+apply wf_var with s.
+
+apply IHIH2 ; auto with coc core.
+apply IHIH5 ; auto with coc core.
+apply wf_var with s.
+apply IHIH3 ; auto with coc core.
+
+apply IHIH6 ; auto with coc core.
+apply wf_var with s.
+apply IHIH2 ; auto with coc core.
+
+apply coerce_sum with s ; auto with coc.
+
+apply IHIH4 ; auto with coc.
+apply wf_var with s.
+apply IHIH3 ; auto with coc core.
+apply IHIH5 ; auto with coc core.
+apply wf_var with s.
+apply IHIH3 ; auto with coc core.
+
+apply IHIH6 ; auto with coc core.
+apply wf_var with s.
+apply IHIH2 ; auto with coc core.
+
+apply coerce_sub_l ; auto with coc core.
+apply IHIH0 ; auto with coc core.
+apply wf_var with set.
+eapply coerce_sort_l  ; auto with coc.
+
+apply coerce_sub_r ; auto with coc core.
+apply IHIH0 ; auto with coc core.
+apply wf_var with set.
+eapply coerce_sort_r  ; auto with coc.
+
+apply coerce_trans with (lift_rec 1 B n) ; auto with coc core.
+Qed.
 
   Theorem thinning :
    forall e t T,
    typ e t T -> forall A, wf (A :: e) -> typ (A :: e) (lift 1 t) (lift 1 T).
+Proof.
 unfold lift in |- *.
 intros.
 inversion_clear H0.
@@ -204,19 +262,21 @@ apply wf_var with s; auto with coc core arith datatypes.
 Qed.
 
 Theorem thinning_coerce : 
-   forall e T U,
-   e |- T >> U -> 
-   forall A, wf (A :: e) -> (A :: e) |- (lift 1 T) >> (lift 1 U).
+   forall e T U s,
+   e |- T >> U : s ->
+   forall A, wf (A :: e) -> (A :: e) |- (lift 1 T) >> (lift 1 U) : s.
+Proof.
 unfold lift ; intros.
 inversion_clear H0.
 apply coerce_weak_weak with A e; auto with coc core arith datatypes.
-apply wf_var with s; auto with coc core arith datatypes.
+apply wf_var with s0; auto with coc core arith datatypes.
 Qed.
 
-  Lemma thinning_n :
+Lemma thinning_n :
    forall n e f,
    trunc _ n e f ->
    forall t T, typ f t T -> wf e -> typ e (lift n t) (lift n T).
+Proof.
 simple induction n.
 intros.
 rewrite lift0.
@@ -239,10 +299,9 @@ apply typ_wf with x (Srt s); auto with coc core arith datatypes.
 apply wf_var with s; auto with coc core arith datatypes.
 Qed.
 
-  Lemma thinning_n_coerce :
-   forall n e f,
-   trunc _ n e f ->
-   forall T U, f |- T >> U -> wf e -> e |- (lift n T) >> (lift n U).
+Lemma thinning_n_coerce : forall n e f, trunc _ n e f ->
+  forall T U s, f |- T >> U : s -> wf e -> e |- (lift n T) >> (lift n U) : s.
+Proof.
 simple induction n.
 intros.
 rewrite lift0.
@@ -250,7 +309,7 @@ rewrite lift0.
 replace e with f; auto with coc core arith datatypes.
 inversion_clear H; auto with coc core arith datatypes.
 
-do 8 intro.
+do 9 intro.
 inversion_clear H0.
 intro.
 rewrite simpl_lift; auto with coc core arith datatypes.
@@ -259,10 +318,10 @@ rewrite simpl_lift; auto with coc core arith datatypes.
 inversion_clear H0.
 replace (lift (S n0) U) with (lift 1 (lift n0 U)).
 apply thinning_coerce; auto with coc core arith datatypes.
-apply H with f; auto with coc core arith datatypes.
-apply typ_wf with x (Srt s); auto with coc core arith datatypes.
+eapply H with f ; auto with coc core arith datatypes.
+apply typ_wf with x (Srt s0); auto with coc core arith datatypes.
 
-apply wf_var with s; auto with coc core arith datatypes.
+apply wf_var with s0; auto with coc core arith datatypes.
 rewrite <- simpl_lift.
 auto.
 Qed.
